Add helper function for `Fin` reduction and docs

Polylean/Experiments/GeneralAbelianGroup.lean
@@ -1,83 +1,46 @@
 import Polylean.FreeAbelianGroup
 import Polylean.Experiments.AddTree
 
-section defs
+section ArraysAndLists
 
-def pow_times (T : Type _) : ℕ → Type _
-  | Nat.zero => Unit
-  | Nat.succ n => T × (pow_times T n)
-
-instance : Pow (Type _) ℕ where
-    pow := pow_times
-
-def pow_sum (T : Type _) : ℕ → Type _
-  | Nat.zero => Empty
-  | Nat.succ n => T ⊕ (pow_sum T n)
-
-section arrays_lists
-
--- def Array.get' {α : Type _} (a : Array α) {n : ℕ} (h : a.size = n) (i : ℕ) (hi : i < n) : α :=
---  Array.get a ⟨i, Eq.substr h hi⟩
-
-section get'
-
-variable {α : Type _} (l : List α) {n : ℕ} (h : l.length = n)
-
-def List.get' (i : ℕ) (hi : i < n) : α :=
-  List.get l ⟨i, Eq.substr h hi⟩
-
-@[simp] theorem List.get'_zero (hi : Nat.zero < n) : l.get' h Nat.zero hi = l.head (List.ne_nil_of_length_pos (Eq.substr h hi)) := by
-  match l with
-    | nil => subst h; contradiction
-    | cons _ _ => rfl
-
--- theorem List.get'_succ (hd : α) (tl : List α) (hyp_len : (hd :: tl).length = n) (i : ℕ) (hi : Nat.succ i < n) : (hd :: tl).get' hyp_len i.succ hi =
---  tl.get' _ i _ := sorry
-
-end get'
-
-@[simp] theorem Array.dataarray {A : Type _} (a : Array A) : a.data.toArray = a := by
-  sorry
-
-@[simp] theorem List.arraydata {A : Type _} (l : List A) : l.toArray.data = l := sorry
-
-@[simp] theorem List.arraylist {A : Type _} (l : List A) : l.toArray.toList = l := by
+-- a lemma about the `toArrayAux` function needed for the next theorem
+lemma List.aux_append {α : Type _} (l : List α) : ∀ l' : List α, List.toArrayAux l {data := l'} = {data := l' ++ l} := by
   induction l with
-    | nil => rfl
-    | cons _ _ ih =>
-      sorry
+    | nil =>
+      intro
+      simp [toArrayAux]
+    | cons h t ih =>
+      intro l'
+      simp [toArrayAux, Array.push, concat]
+      rw [ih (concat l' h)]
+      simp
+      let rec concat_append : ∀ (a : α) (l₁ l₂ : List α), concat l₁ a ++ l₂ = l₁ ++ (a :: l₂) := sorry
+      apply concat_append
 
-@[simp] theorem Array.listarray {A : Type _} (a : Array A) : a.toList.toArray = a := by
-  match a with
-    | ⟨l⟩ =>
-      -- apply congrArg Array.mk
-      induction l with
-        | nil => rfl
-        | cons _ _ ih =>
-          -- [toList, foldr]
-          sorry
+-- converting a list to an array and then extracting the data preserves the list
+@[simp] theorem List.arraydata {A : Type _} (l : List A) : l.toArray.data = l := by
+  rw [toArray, Array.mkEmpty, List.aux_append]
+  simp
 
+-- the size of a list is preserved when coverted to an array and back
 @[simp] theorem List.arraysize {α : Type _} (l : List α) : l.toArray.size = l.length := by
   rw [Array.size, arraydata]
 
-def Array.get' {α : Type _} (a : Array α) {n : ℕ} (h : a.size = n) (i : ℕ) (hi : i < n) : α :=
-  a.data.get' h i hi
+-- a helper lemma for solving rewriting issues with `Fin`
+theorem List.get_index_eq : {l l' : List α} → (hl : l = l') → (i : ℕ) → (bnd : i < l.length) → l.get ⟨i, bnd⟩ = l'.get ⟨i, hl ▸ bnd⟩
+  | _, _, rfl, _, _ => rfl
 
+-- getting the `i`th element of an array is the same as getting the `i`th element of the corresponding list
 @[simp] theorem Array.getfromlist : (l : List T)  → (i : ℕ) → (h : i < l.length) → Array.get (l.toArray) ⟨i, Eq.substr l.arraysize h⟩ = l.get ⟨i, h⟩
   | List.nil, _, h => by contradiction
-  | List.cons hd tl, Nat.zero, _ => by simp [get]; sorry
-  | List.cons _ _, Nat.succ m, h => by rw [List.get]; admit
-
-theorem Array.get'fromlist : (l : List T) → {n : ℕ} → (i : ℕ) → (h : l.length = n) → (hi : i < n) → Array.get' (l.toArray) (by rw [List.arraysize]; exact h) i hi = l.get' h i hi
-  | List.cons hd tl, _, Nat.zero, rfl, hi => by
-    rw [List.get'_zero, Array.get', List.get'_zero]
-    sorry
-  | List.cons _ _, _, Nat.succ j, h, hi => sorry
+  | List.cons hd tl, Nat.zero, _ => by rw [get, List.get_index_eq (List.arraydata (hd :: tl)), List.get]
+  | List.cons _ _, Nat.succ m, h => by rw [get, List.get_index_eq (List.arraydata _), List.get]
 
 theorem List.maplength {T S : Type _} (ϕ : T → S) : (l : List T) → l.length = (l.map ϕ).length
   | List.nil => rfl
   | List.cons h t => by rw [List.length, List.map, List.length, maplength ϕ t]
 
+-- the value of a function `ϕ` on the `i`th element of a list `l` is the same as the value of the `i`th element of the list `map ϕ l`
 theorem List.mapget {T S : Type _} (ϕ : T → S) : (l : List T) → (i : ℕ) → (h : i < List.length l) → ϕ (l.get ⟨i, h⟩) = (l.map ϕ).get ⟨i, Eq.subst (maplength ϕ l) h⟩
   | List.nil, _, _ => by contradiction
   | List.cons _ _, Nat.zero, _ => by simp [get, map]
@@ -87,7 +50,23 @@ def List.mapcomp (ϕ : T → S) (ψ : S → R) : (l : List T) → List.map ψ (L
   | nil => rfl
   | cons _ l' => by simp only [map]; rw [mapcomp _ _ l']; rfl
 
-end arrays_lists
+end ArraysAndLists
+
+section Defs
+
+-- iterated product
+def pow_times (T : Type _) : ℕ → Type _
+  | Nat.zero => Unit
+  | Nat.succ n => T × (pow_times T n)
+
+instance : Pow (Type _) ℕ where
+    pow := pow_times
+
+-- iterated direct sums
+def pow_sum (T : Type _) : ℕ → Type _
+  | Nat.zero => Empty
+  | Nat.succ n => T ⊕ (pow_sum T n)
+
 
 instance : AddCommGroup Unit :=
   {
@@ -111,6 +90,7 @@ def ℤpowgroup : (n : ℕ) → AddCommGroup (ℤ ^ n)
     | Nat.zero => inferInstanceAs (AddCommGroup Unit)
     | Nat.succ n => @DirectSum.directSum ℤ (pow_times ℤ n) _ (ℤpowgroup n)
 
+-- ℤ^n is a group
 instance ℤgrp (n : ℕ) : AddCommGroup (ℤ ^ n) := ℤpowgroup n
 
 instance (n : ℕ) : AddCommGroup (pow_times ℤ n) := ℤpowgroup n
@@ -129,21 +109,27 @@ match n with
   | Nat.zero => inferInstanceAs (FreeAbelianGroup Unit Empty)
   | Nat.succ n => @prodFree _ _ _ (inferInstanceAs (AddCommGroup (ℤ ^ n))) _ _ _ (ℤpowfreegroup n)
 
+-- ℤ^n is a free Abelian group
 instance ℤfreegrp (n : ℕ) : FreeAbelianGroup (ℤ ^ n) (pow_sum Unit n) := ℤpowfreegroup n
 
 instance (n : ℕ) : FreeAbelianGroup (pow_times ℤ n) (pow_sum Unit n) := ℤpowfreegroup n
 
-def unit_pow_list {T : Type _} {n : ℕ} (l : List T) (h : l.length = n) : pow_sum Unit n → T :=
+-- takes a list of values in `T` of length `n` and returns a function from `Unit ⊕ Unit ⊕ ... n times ... ⊕ Unit → T`
+-- mapping the elements of `pow_sum Unit n` to the corresponding elements of `T` in order
+def unitBasisMap {T : Type _} {n : ℕ} (l : List T) (h : l.length = n) : pow_sum Unit n → T :=
 match n with
   | Nat.zero => Empty.rec _
   | Nat.succ m =>
     match l with
-      | List.cons t l' => λ s => Sum.casesOn s (fun | Unit.unit => t) (unit_pow_list l' (by rw [List.length, ← Nat.succ_eq_add_one] at h; injection h; assumption))
+      | List.cons t l' => λ s => Sum.casesOn s
+                  (fun | Unit.unit => t)
+                  (unitBasisMap l' (by rw [List.length, ← Nat.succ_eq_add_one] at h; injection h; assumption))
 
 def zeros : (n : ℕ) → ℤ ^ n
 | Nat.zero => ()
 | Nat.succ n => Prod.mk (0 : ℤ) (zeros n)
 
+-- returns a basis of `ℤ^n`
 def ℤbasis : (n : ℕ) → List (ℤ ^ n)
 | Nat.zero => List.nil
 | Nat.succ n => List.cons (Prod.mk (1 : ℤ) (zeros n)) (ℤbasis n |>.map ι₂)
@@ -152,16 +138,20 @@ theorem zero_zero : (n : ℕ) → (0 : ℤ ^ n) = (zeros n)
 | Nat.zero => rfl
 | Nat.succ m => by rw [zeros, ← zero_zero m]; rfl
 
-end defs
+end Defs
 
-section
 
-def induced_map {A : Type _} [AddCommGroup A] {n : ℕ} (l : List A) (h : l.length = n) : ℤ^n → A :=
-FreeAbelianGroup.inducedMap A (unit_pow_list l h)
+section InducedFreeMap
 
-instance ind_hom {A : Type _} [AddCommGroup A] {n : ℕ} (l : List A) (h : l.length = n) : AddCommGroup.Homomorphism (induced_map l h) := FreeAbelianGroup.induced_hom A _
+-- the unique map `ϕ : ℤ^n → A` taking the basis elements to the given list of values `l`
+def inducedFreeMap {A : Type _} [AddCommGroup A] {n : ℕ} (l : List A) (h : l.length = n) : ℤ^n → A :=
+FreeAbelianGroup.inducedMap A (unitBasisMap l h)
 
-theorem map_basis {A : Type _} [AddCommGroup A] : {m : ℕ} → (l : List A) → (h : l.length = m) → (List.map (induced_map l h) (ℤbasis m)) = l
+-- the above map is a group homomorphism
+instance ind_hom {A : Type _} [AddCommGroup A] {n : ℕ} (l : List A) (h : l.length = n) : AddCommGroup.Homomorphism (inducedFreeMap l h) := FreeAbelianGroup.induced_hom A _
+
+-- a proof that the above map takes the basis elements to the elements in the list
+theorem map_basis {A : Type _} [AddCommGroup A] : {m : ℕ} → (l : List A) → (h : l.length = m) → (List.map (inducedFreeMap l h) (ℤbasis m)) = l
 | Nat.zero, List.nil, _ => rfl
 | Nat.succ m, List.cons t l', h' => by
   simp [List.map]
@@ -169,18 +159,18 @@ theorem map_basis {A : Type _} [AddCommGroup A] : {m : ℕ} → (l : List A) →
   · have : Prod.mk (1 : ℤ) (zeros m) = (ℤfreegrp (Nat.succ m)).i (Sum.inl () : Unit ⊕ (pow_sum Unit m)) := by
       rw [← zero_zero, FreeAbelianGroup.left_incl]; apply congrArg; rfl
     rw [this]
-    apply ( congrFun ((ℤfreegrp (Nat.succ m)).induced_extends (unit_pow_list (List.cons t l') h')) (Sum.inl ()) )
+    apply ( congrFun ((ℤfreegrp (Nat.succ m)).induced_extends (unitBasisMap (List.cons t l') h')) (Sum.inl ()) )
   · have h'' := h'
     rw [List.length, Nat.add_one, Nat.succ_inj'] at h''
     have ih := map_basis l' h''
-    have ind_cons : induced_map (t :: l') h' ∘ ι₂ = induced_map l' h'' := by
-      rw [induced_map, induced_map]
-      have : (unit_pow_list l' h'') = (unit_pow_list (List.cons t l') h') ∘ Sum.inr := by apply funext; intro; simp [unit_pow_list]
+    have ind_cons : inducedFreeMap (t :: l') h' ∘ ι₂ = inducedFreeMap l' h'' := by
+      rw [inducedFreeMap, inducedFreeMap]
+      have : (unitBasisMap l' h'') = (unitBasisMap (List.cons t l') h') ∘ Sum.inr := by apply funext; intro; simp [unitBasisMap]
       rw [this, FreeAbelianGroup.induced_right]
     rw [ind_cons]
     exact ih
 
-end
+end InducedFreeMap
 
 
 section AddTreeGroup
@@ -188,6 +178,8 @@ section AddTreeGroup
 variable (t : IndexAddTree)
 variable {A : Type _} [AddCommGroup A] [Repr A]
 variable {n : ℕ} (l : List A) (h : l.length = n) (hpos : n > 0) -- basisImages
+
+-- a few helper results and lemmas
 
 instance prodrepr (A B : Type _) [Repr A] [Repr B] : Repr (A × B) := inferInstance
 
@@ -201,68 +193,71 @@ lemma larrlengthpos : Array.size (List.toArray l) > 0 := by
   rw [GT.gt, List.arraysize, h]
   exact hpos
 
-lemma ℤbasisarrlengthpos : Array.size (List.toArray (ℤbasis n)) > 0 := by
-  rw [GT.gt, List.arraysize]
-  let rec ℤbasislen : ∀ m : ℕ, List.length (ℤbasis m) = m
+def ℤbasislen : ∀ m : ℕ, List.length (ℤbasis m) = m
     | Nat.zero => rfl
     | Nat.succ m' => by rw [ℤbasis, List.length, Nat.add_one, ← List.maplength, ℤbasislen m']
+
+lemma ℤbasisarrlengthpos : Array.size (List.toArray (ℤbasis n)) > 0 := by
+  rw [GT.gt, List.arraysize]
   rw [ℤbasislen]
   assumption
 
--- set_option pp.all true
-theorem array_get'_index_eq (hl : l.toArray.size = n) (hℤb : (ℤbasis n).toArray.size = n) (i : ℕ) (hi : i < n) :
-  Array.get' (List.toArray l) hl i hi =
-    induced_map l h (Array.get' (List.toArray (ℤbasis n)) hℤb i hi) := by
-    rw [Array.getfromlist, Array.getfromlist, List.mapget (induced_map l h)]
-    have : i < List.length (List.map (induced_map l h) (ℤbasis n)) ↔ i < n := sorry
-    rw [this]
-
+-- taking an abstract tree to a given list of `n` elements of group `A` is equivalent to
+-- first taking it to the basis of `ℤ^n` and then apply the `inducedFreeMap`
 theorem IndexAddTree.trees_consistent : IndexAddTree.foldMap t l.toArray (larrlengthpos l h hpos) =
-                         (induced_map l h) (IndexAddTree.foldMap t (ℤbasis n).toArray (ℤbasisarrlengthpos hpos)) := by
+                         (inducedFreeMap l h) (IndexAddTree.foldMap t (ℤbasis n).toArray (ℤbasisarrlengthpos hpos)) := by
   induction t with
-    | leaf a =>
-      simp [foldMap]
-      rw [Array.getfromlist, Array.getfromlist, List.mapget (induced_map l h)]
-      have := map_basis l h
-      sorry
-      -- apply congrArg
-      sorry
-    | negLeaf a =>
-      simp [foldMap]
-      apply congrArg
-      rw [Array.getfromlist, Array.getfromlist, List.mapget (induced_map l h)]
-      have := map_basis l h
-      simp [this]
-      sorry
+    | leaf _ =>
+        simp [foldMap]
+        rw [Array.getfromlist, Array.getfromlist, List.mapget (inducedFreeMap l h), List.get_index_eq (map_basis l h)]
+        apply congrArg
+        -- apply Fin.eq_of_val_eq
+        all_goals sorry
+    | negLeaf _ =>
+        simp [foldMap]
+        apply congrArg
+        rw [Array.getfromlist, Array.getfromlist, List.mapget (inducedFreeMap l h), List.get_index_eq (map_basis l h)]
+        apply congrArg
+        apply Fin.eq_of_val_eq
+        simp
+        subst h
+        all_goals sorry
     | node _ _ ihl ihr => simp [ihl, ihr, foldMap]
     | subNode _ _ ihl ihr => simp [ihl, ihr, foldMap]
 
 end AddTreeGroup
 
 /-
-section formalexample
+section FormalExample
 
-def n : ℕ := 3
+abbrev n : ℕ := 3
 
-open Vector in
-def ν {A : Type _} [AddCommGroup A] (v : Vector A n) :=
-    match v with
-      | cons x (cons y (cons z nil)) => x + (y - z) + z - x = y
+open List in
+def ν {A : Type _} [AddCommGroup A] (l : List A) (h : l.length = n) : Prop :=
+    match l, h with
+      | (cons x (cons y (cons z nil))), rfl => x + (y - z) + z - x = y
 
-theorem valid_iff_free_basis : (∀ {A : Type _} [AddCommGroup A], ∀ v : Vector A n, ν v) ↔ (ν (ℤbasis n)) := by
+theorem valid_iff_free_basis : (∀ {A : Type} [AddCommGroup A], ∀ (l : List A) (h : l.length = n), ν l h) ↔ (ν (ℤbasis n) (ℤbasislen n)) := by
   apply Iff.intro
-  · intro h
-    apply h
-  · intro h
-    intro A _ v
-    have ϕ := induced_map v
-    have := congrArg ϕ h
-    simp only [ι₁, ι₂, zeros] at this
-    simp only [AddCommGroup.Homomorphism.add_dist] at this
-    sorry
+  · intro hyp
+    exact hyp (ℤbasis n) (ℤbasislen n)
+  · intro hyp
+    intro A _ l h
+    let ϕ := induced_map l rfl
+    have basismap := map_basis l rfl
+    match l, h with
+      | List.cons a (List.cons b (List.cons c List.nil)), rfl =>
+        simp [ν, ℤbasis] at hyp
+        have ϕmap := congrArg ϕ hyp
+        simp at ϕmap
+        simp only [ι₁, ι₂, zeros] at ϕmap
+        simp [List.map, ℤbasis, ι₁, ι₂, zeros, unit_pow_list, h, map_basis] at basismap
+        let ⟨ha, hb, hc⟩ := basismap
+        simp [ha, hb, hc] at ϕmap
 
-theorem eqn_valid {A : Type _} [AddCommGroup A] : ∀ v : Vector A n, ν v :=
+
+theorem eqn_valid {A : Type} [AddCommGroup A] : ∀ (l : List A) (h : l.length = n), ν l h :=
   (Iff.mpr valid_iff_free_basis) rfl
 
-end formalexample
+end FormalExample
 -/
